cogent/examples/repeat/RepeatShallow.thy
@@ -4,80 +4,80 @@ begin
 
 section "Repeat"
 
-fun repeatatl :: "nat \<Rightarrow> ('a \<Rightarrow> 'b \<Rightarrow> bool) \<Rightarrow> ('a \<Rightarrow> 'b \<Rightarrow> 'a) \<Rightarrow> 'a \<Rightarrow> 'b \<Rightarrow> 'a"
+fun repeatatm :: "nat \<Rightarrow> ('a \<Rightarrow> 'b \<Rightarrow> bool) \<Rightarrow> ('a \<Rightarrow> 'b \<Rightarrow> 'a) \<Rightarrow> 'a \<Rightarrow> 'b \<Rightarrow> 'a"
   where
-"repeatatl 0 _ _ acc _ = acc" |
-"repeatatl (Suc n) f g acc obsv = (if f acc obsv then acc else repeatatl n f g (g acc obsv) obsv)"
+"repeatatm 0 _ _ acc _ = acc" |
+"repeatatm (Suc n) f g acc obsv = (if f acc obsv then acc else repeatatm n f g (g acc obsv) obsv)"
 
-declare repeatatl.simps[simp del]
+declare repeatatm.simps[simp del]
 
 subsection "Step and early termination lemmas"
 
-lemma repeatatl_step_stop_Suc:
-  "f (repeatatl n f g a b) b 
-    \<Longrightarrow> repeatatl (Suc n) f g a b = repeatatl n f g a b"
+lemma repeatatm_step_stop_Suc:
+  "f (repeatatm n f g a b) b 
+    \<Longrightarrow> repeatatm (Suc n) f g a b = repeatatm n f g a b"
   apply (induct n arbitrary: a)
-   apply (simp add: repeatatl.simps)
-  apply (subst repeatatl.simps)
+   apply (simp add: repeatatm.simps)
+  apply (subst repeatatm.simps)
   apply clarsimp
-  apply (rule conjI, simp add: repeatatl.simps, clarsimp)
+  apply (rule conjI, simp add: repeatatm.simps, clarsimp)
   apply (rule sym)
-  apply (subst repeatatl.simps)
+  apply (subst repeatatm.simps)
   apply clarsimp
-  apply (rotate_tac 1, subst (asm) repeatatl.simps)
+  apply (rotate_tac 1, subst (asm) repeatatm.simps)
   apply clarsimp
   done
 
-lemma repeatatl_step:
-  "\<not>f (repeatatl n f g a b) b 
-    \<Longrightarrow> repeatatl (Suc n) f g a b = g (repeatatl n f g a b) b"
+lemma repeatatm_step:
+  "\<not>f (repeatatm n f g a b) b 
+    \<Longrightarrow> repeatatm (Suc n) f g a b = g (repeatatm n f g a b) b"
   apply (induct n arbitrary: a)
-   apply (simp add: repeatatl.simps)
-  apply (subst repeatatl.simps)
+   apply (simp add: repeatatm.simps)
+  apply (subst repeatatm.simps)
   apply clarsimp
-  apply (rule conjI, simp add: repeatatl.simps, clarsimp, clarsimp)
+  apply (rule conjI, simp add: repeatatm.simps, clarsimp, clarsimp)
   apply (rule sym)
-  apply (subst repeatatl.simps)
+  apply (subst repeatatm.simps)
   apply clarsimp
-  apply (rotate_tac 1, subst (asm) repeatatl.simps)
+  apply (rotate_tac 1, subst (asm) repeatatm.simps)
   apply clarsimp
   done
 
-lemma repeatatl_stop_Suc:
-  "\<lbrakk>f (repeatatl n f g a b) b\<rbrakk> \<Longrightarrow> f (repeatatl (Suc n) f g a b) b"
+lemma repeatatm_stop_Suc:
+  "\<lbrakk>f (repeatatm n f g a b) b\<rbrakk> \<Longrightarrow> f (repeatatm (Suc n) f g a b) b"
   apply (induct n arbitrary: a)
-   apply (simp add: repeatatl.simps)
-  apply (subst repeatatl.simps)
+   apply (simp add: repeatatm.simps)
+  apply (subst repeatatm.simps)
   apply clarsimp
-  apply (rotate_tac 1, subst (asm) repeatatl.simps)
+  apply (rotate_tac 1, subst (asm) repeatatm.simps)
   apply clarsimp
   done
 
-lemma repeatatl_stop:
-  "\<lbrakk>f (repeatatl n f g a b) b; n \<le> m\<rbrakk> \<Longrightarrow> f (repeatatl m f g a b) b"
+lemma repeatatm_stop:
+  "\<lbrakk>f (repeatatm n f g a b) b; n \<le> m\<rbrakk> \<Longrightarrow> f (repeatatm m f g a b) b"
   apply (induct m arbitrary: a n)
    apply simp
   apply (case_tac "n < Suc m")
-   apply (rule_tac f = f in repeatatl_stop_Suc)
+   apply (rule_tac f = f in repeatatm_stop_Suc)
    apply clarsimp
   apply clarsimp
   done
 
-lemma repeatatl_step_stop:
-  "\<lbrakk>f (repeatatl n f g a b) b; n \<le> m\<rbrakk> \<Longrightarrow> repeatatl m f g a b = repeatatl n f g a b"
+lemma repeatatm_step_stop:
+  "\<lbrakk>f (repeatatm n f g a b) b; n \<le> m\<rbrakk> \<Longrightarrow> repeatatm m f g a b = repeatatm n f g a b"
   apply (induct m arbitrary: a n)
    apply simp
   apply (case_tac "n < Suc m")
-   apply (subst repeatatl_step_stop_Suc)
+   apply (subst repeatatm_step_stop_Suc)
     apply clarsimp
    apply clarsimp
   apply clarsimp
   done
 
-lemma repeatatl_not_stop_Suc:
-  "\<not>f (repeatatl (Suc n) f g a b) b \<Longrightarrow> \<not>f (repeatatl n f g a b) b"
-  apply (rule_tac Q = "f (repeatatl (Suc n) f g a b) b" in  contrapos_nn; simp)
-  apply (cut_tac n = n and f = f and g = g and a = a and b = b in repeatatl_stop_Suc; simp)
+lemma repeatatm_not_stop_Suc:
+  "\<not>f (repeatatm (Suc n) f g a b) b \<Longrightarrow> \<not>f (repeatatm n f g a b) b"
+  apply (rule_tac Q = "f (repeatatm (Suc n) f g a b) b" in  contrapos_nn; simp)
+  apply (cut_tac n = n and f = f and g = g and a = a and b = b in repeatatm_stop_Suc; simp)
   done
 
 end
