cogent/examples/repeat/WordArrayMono.thy
@@ -52,4 +52,24 @@ lemma (in WordArrayValue) vwa_put_monoexpr_correct:
   apply (clarsimp simp: rename_monoval_no_vfuns[THEN no_vfuns_rename_monoval] rename_monoval_no_vfuns)
   done
 
+subsection "wordarray_get_opt"
+
+lemma (in WordArrayValue) vwa_get_opt_monoexpr_correct:
+  "\<And>v v'.
+       vwa_get_opt (rename_val rename' (monoval v)) v'
+       \<Longrightarrow> \<exists>v''. v' = rename_val rename' (monoval v'') \<and> vwa_get_opt v v''"
+  apply (clarsimp simp: vwa_get_opt_def)
+  apply (case_tac v; clarsimp)
+  apply (rename_tac v' t xs i z za)
+  apply (case_tac z; clarsimp)
+  apply (case_tac za; clarsimp)
+  apply (clarsimp split: if_splits)
+   apply (rule_tac x = " VSum ''Something'' (xs ! unat i)" in exI)
+   apply (clarsimp simp: no_vfuns_rename_monoval)
+   apply fastforce
+  apply (rule_tac x = "VSum ''Nothing'' VUnit" in exI)
+  apply (clarsimp simp: no_vfuns_rename_monoval)
+  apply (rule exI, rule exI, rule_tac x = i in exI, intro exI conjI impI; simp?)
+  done
+
 end
